authentication complete

ModularEngine/src/LogicEngine.FStar/authenticate.fst
@@ -8,7 +8,6 @@ type message :: _ =  fun ('P::principal => principal => polyterm => E) =>
         pto:principal *
           i:polyterm{'P pfrom pto i}))
 
-type Says :: principal => polyterm => E
 type trivial :: _ = (fun (p:principal) (q:principal) (i:polyterm) => True)
 type jmessage = message (fun (p:principal) (q:principal) (i:polyterm) => (Says p i)) 
 type msg = 
@@ -22,28 +21,61 @@ val lookup_my_credentials : unit -> (p:principal{IsMe p} * pk p * sk p)
 val lookup_pubkey: p:principal -> option (pk p)
 let myKeys = lookup_my_credentials ()
 
-val infon2bytes: i:polyterm -> b:bytes{Serialized i b}
-(* let infon2bytes i =  *)
-(*   let str = printInfon i in  *)
-(*     FromUnicodeString str  *)
+val polyterm2bytes: i:polyterm -> b:bytes{Serialized i b}
+let polyterm2bytes i =
+  let str = printInfon i in
+    FromUnicodeString str
 
 val msg2bytes: msg -> bytes
-(* let msg2bytes msg =  *)
-(*   let (me, pkey, skey) = myKeys in  *)
-(*     match msg with  *)
-(*       | Forwarded((p, q, i)) -> infon2bytes i *)
+let msg2bytes m =
+  let (me, pkey, skey) = myKeys in
+    match m with
+      | Forwarded ((p,q,i)) -> polyterm2bytes i
 
-(*       | Justified((p, q, i)) when p=me ->  *)
-(*           assert (Says me i); *)
-(*           let b = infon2bytes i in  *)
-(*           let dsig = rsa_sign me skey i b in *)
-(*           let ji = App JustifiedInfon [i; (App SignatureEvidence [p; i; dsig])] in  *)
-(*             infon2bytes ji *)
+      | Justified((p, q, i)) when p=me ->
+          assert (Says me i);
+          let b = polyterm2bytes i in
+          let dsig = rsa_sign me skey i b in
+          let ji = JustifiedPoly (Const (PrincipalConstant p)) i (Const (Bytes dsig)) in 
+            polyterm2bytes ji
 
-val b2s: b:bytes -> s:string{Net.Received b => Net.Received s}
-val bytes2infon: b:bytes -> option (i:polyterm{Net.Received b => Net.Received i})
-(* let bytes2infon b =  *)
-(*   let str = ToUnicodeString b in  *)
-(*   let i = parseInfon i  *)
-  
+val checkMono : i:term -> b:bool{b=true => CheckedInfonMono i}
+let rec checkMono i = match i with 
+  | Var x -> true
+  | Const c -> true
+  | SubstrateQueryTerm _ -> true
+  | App f tms -> 
+      if f=JustifiedInfon then 
+        match tms with 
+          | [(Const (PrincipalConstant p)); i; (Const (Bytes ds))] -> 
+              (match lookup_pubkey p with 
+                 | None -> false
+                 | Some pubk -> 
+                     let bi = polyterm2bytes (MonoTerm i) in 
+                       (rsa_verify p pubk (MonoTerm i) bi ds) && checkMono i)
+          | _ -> false
+      else for_all<term, CheckedInfonMono> checkMono tms 
+        
+val checkInfon : p:polyterm -> b:bool{b=true => CheckedInfon p}
+let rec checkInfon p = match p with
+  | MonoTerm i -> checkMono i
+  | ForallT xs i -> checkMono i
+  | JustifiedPoly (Const (PrincipalConstant p)) i (Const (Bytes ds)) -> 
+      (match lookup_pubkey p with 
+         | None -> false
+         | Some pubk -> 
+             let bi = polyterm2bytes i in 
+               (rsa_verify p pubk i bi ds) && checkInfon i)
+  | _ -> false
 
+val bytes2infon: b:bytes -> option (i:infon{(Net.Received b => Net.Received i)})
+let bytes2infon b = 
+  let s = ToUnicodeString b in 
+    assert (Net.Received b => Net.Received s); 
+    match parseInfon s with 
+      | Some poly when checkInfon poly -> 
+          assert ((ReprPoly poly)=s);
+          assert (Net.Received s => Net.Received poly);
+            Some poly
+      | _ -> None
+    
