ModularEngine/src/LogicEngine.FStar/state.fst
@@ -4,7 +4,7 @@ open Types
 private val infos : Ref infostrate
 let infos = newref []
 
-val addToInfostrate : i:polyterm{Knows i} -> unit
+val addToInfostrate : i:infon{Knows i} -> unit
 let addToInfostrate i = infos := i::!infos
 
 val getInfostrate : unit -> infostrate
